Reduction module.

Code/HOL_Light/Lambda/rules.ml
@@ -1,3 +1,14 @@
+(* ========================================================================= *)
+(*  Initial semantics based on De Brujin encoding                            *)
+(*  with dbmonads and their modules.                                         *)
+(*                                                                           *)
+(*  (c) Copyright, Marco Maggesi 2005 2006 2017, 2020                        *)
+(* ========================================================================= *)
+
+(* ------------------------------------------------------------------------- *)
+(* Inductive datatype of the reduction rules of lambda calculus.             *)
+(* ------------------------------------------------------------------------- *)
+
 let lcrel_INDUCT,lcrel_RECUR = define_type
   "lcrel = LCREL_REFL dblambda
          | LCREL_TRANS lcrel lcrel
@@ -7,29 +18,46 @@ let lcrel_INDUCT,lcrel_RECUR = define_type
          | LCREL_ETA dblambda";;
 
 let RED_RULES,RED_INDUCT,RED_CASES = new_inductive_definition
-  `(!x. RED x x (LCREL_REFL x)) /\
-   (!x y z r s. RED x y r /\ RED y z s ==> RED x z (LCREL_TRANS r s)) /\
-   (!x1 x2 y1 y2 r1 r2. RED x1 y1 r1 /\ RED x2 y2 r2
-      ==> RED (APP x1 x2) (APP y1 y2) (LCREL_APP r1 r2)) /\
-   (!x y r. RED x y r ==> RED (ABS x) (ABS y) (LCREL_ABS r)) /\
-   (!x y. RED (APP (ABS x) y) (SUBST (PUSHENV y REF) x) (LCREL_BETA x y)) /\
-   (!x. RED (ABS (APP (REINDEX SUC x) (REF 0))) x (LCREL_ETA x))`;;
+  `(!x. RED (x,x,LCREL_REFL x)) /\
+   (!x y z r s. RED (x,y,r) /\ RED (y,z,s) ==> RED (x,z,LCREL_TRANS r s)) /\
+   (!x1 x2 y1 y2 r1 r2. RED (x1,y1,r1) /\ RED (x2,y2,r2)
+      ==> RED (APP x1 x2, APP y1 y2, LCREL_APP r1 r2)) /\
+   (!x y r. RED (x,y,r) ==> RED (ABS x, ABS y, LCREL_ABS r)) /\
+   (!x y. RED (APP (ABS x) y, SUBST (PUSHENV y REF) x, LCREL_BETA x y)) /\
+   (!x. RED (ABS (APP (REINDEX SUC x) (REF 0)), x, LCREL_ETA x))`;;
 
 let [RED_REFL;RED_TRANS;RED_APP;RED_ABS;RED_BETA;RED_ETA] =
   CONJUNCTS RED_RULES;;
 
-let RED_INDUCT_STRONG = derive_strong_induction (RED_RULES,RED_INDUCT);;
+let RED_INDUCT_ALT = prove
+ (`!P. (!x. P x x (LCREL_REFL x)) /\
+       (!x y z r s.
+            P x y r /\ P y z s ==> P x z (LCREL_TRANS r s)) /\
+       (!x1 x2 y1 y2 r1 r2.
+            P x1 y1 r1 /\ P x2 y2 r2
+            ==> P (APP x1 x2) (APP y1 y2) (LCREL_APP r1 r2)) /\
+       (!x y r. P x y r ==> P (ABS x) (ABS y) (LCREL_ABS r)) /\
+       (!x y.
+            P (APP (ABS x) y) (SUBST (PUSHENV y REF) x) (LCREL_BETA x y)) /\
+       (!x. P (ABS (APP (REINDEX SUC x) (REF 0))) x (LCREL_ETA x))
+       ==> (!x y r. RED (x,y,r) ==> P x y r)`,
+  GEN_TAC THEN STRIP_TAC THEN
+  SUBGOAL_THEN `!t. RED t ==> let x,y,r = t in P x y r` MP_TAC THENL
+  [MATCH_MP_TAC RED_INDUCT THEN REPEAT STRIP_TAC THEN CONV_TAC let_CONV THEN
+   REPEAT (FIRST_X_ASSUM (MP_TAC o CONV_RULE let_CONV)) THEN ASM_MESON_TAC[];
+   REWRITE_TAC[FORALL_PAIR_THM]] THEN
+  CONV_TAC (ONCE_DEPTH_CONV let_CONV) THEN MESON_TAC[]);;
 
 let RED_IMP_LC_REL = prove
- (`!x y r. RED x y r ==> REDREL x y`,
-  MATCH_MP_TAC RED_INDUCT THEN REWRITE_TAC[REDREL_RULES] THEN
+ (`!x y r. RED (x,y,r) ==> REDREL x y`,
+  MATCH_MP_TAC RED_INDUCT_ALT THEN REWRITE_TAC[REDREL_RULES] THEN
   CONJ_TAC THEN REPEAT GEN_TAC THENL
   [MATCH_MP_TAC REDREL_BETA; MATCH_MP_TAC REDREL_ETA] THEN
   REWRITE_TAC[DBLAMBDA_BETA_RULES; DBLAMBDA_ETA_RULES]);;
 
 let REDREL_EQ_RED = prove
- (`!x y. REDREL x y <=> ?r. RED x y r`,
-  SUBGOAL_THEN `!x y. REDREL x y ==> ?r. RED x y r`
+ (`!x y. REDREL x y <=> ?r. RED (x,y,r)`,
+  SUBGOAL_THEN `!x y. REDREL x y ==> ?r. RED (x,y,r)`
    (fun th -> MESON_TAC[th; RED_IMP_LC_REL]) THEN
   MATCH_MP_TAC REDREL_INDUCT THEN CONJ_TAC THENL
   [MATCH_MP_TAC DBLAMBDA_BETA_INDUCT THEN GEN_TAC THEN GEN_TAC THEN
@@ -58,9 +86,13 @@ let RED2 = new_recursive_definition lcrel_RECUR
    (!x. RED2 (LCREL_ETA x) = x)`;;
 
 let RED_PROJECTIONS = prove
- (`!x y r. RED x y r ==> RED1 r = x /\ RED2 r = y`,
-  MATCH_MP_TAC RED_INDUCT THEN REPEAT STRIP_TAC THEN
+ (`!x y r. RED (x,y,r) ==> RED1 r = x /\ RED2 r = y`,
+  MATCH_MP_TAC RED_INDUCT_ALT THEN REPEAT STRIP_TAC THEN
   ASM_REWRITE_TAC[RED1; RED2]);;
+
+(* ------------------------------------------------------------------------- *)
+(* Reduction relation.                                                       *)
+(* ------------------------------------------------------------------------- *)
 
 let RFREES_RULES,RFREES_INDUCT,RFREES_CASES = new_inductive_set
   `(!i x. i IN FREES x ==> i IN RFREES (LCREL_REFL x)) /\
@@ -95,6 +127,10 @@ let RFREES_CLAUSES = prove
    (!r s x. RFREES (LCREL_BETA x y) = {i | SUC i IN FREES x} UNION FREES y) /\
    (!r s x. RFREES (LCREL_ETA x) = FREES x)`,
   REWRITE_TAC[EXTENSION; RFREES_INVERSION] THEN SET_TAC[]);;
+
+(* ------------------------------------------------------------------------- *)
+(* Module structure of the reduction relations. *)
+(* ------------------------------------------------------------------------- *)
 
 let RSUBST = new_recursive_definition lcrel_RECUR
   `(!f x. RSUBST f (LCREL_REFL x) = LCREL_REFL (SUBST f x)) /\
@@ -139,8 +175,7 @@ let SUBST_RED2 = prove
   REWRITE_TAC[SUBST_SUBST; SUBST_EXTENS; o_THM; SUBST_DERIV] THEN
   GEN_TAC THEN DISCH_TAC THEN STRUCT_CASES_TAC (SPEC `i:num` num_CASES) THEN
   REWRITE_TAC[DERIV; PUSHENV; SUBST; SUBST_REINDEX] THEN
-  MATCH_MP_TAC EQ_SYM THEN
-  REWRITE_TAC[SUBST_REF_EQ; o_THM; PUSHENV]);;
+  MATCH_MP_TAC EQ_SYM THEN REWRITE_TAC[SUBST_REF_EQ; o_THM; PUSHENV]);;
 
 let MODULE_RSUBST = prove
  (`MODULE SUBST RSUBST`,
@@ -159,3 +194,177 @@ let MODULE_MOR_RED1 = prove
 let MODULE_MOR_RED2 = prove
  (`MODULE_MOR SUBST RSUBST SUBST RED2`,
   REWRITE_TAC[MODULE_MOR; MODULE_RSUBST; MODULE_SUBST; SUBST_RED2]);;
+
+(* ------------------------------------------------------------------------- *)
+(* Reduction module.                                                         *)
+(* ------------------------------------------------------------------------- *)
+
+let red_tybij =
+  let eth = prove
+   (`?t. RED t`,
+    EXISTS_TAC `REF 0, REF 0, LCREL_REFL (REF 0)` THEN
+    REWRITE_TAC[RED_REFL]) in
+  new_type_definition "red" ("MK_RED","DEST_RED") eth;;
+
+let MK_DEST_RED = prove
+ (`!t. MK_RED (DEST_RED t) = t`,
+  REWRITE_TAC[red_tybij]);;
+
+let DEST_MK_RED_EQ = prove
+ (`!t. DEST_RED (MK_RED t) = t <=> RED t`,
+  REWRITE_TAC[red_tybij]);;
+
+let DEST_MK_RED = prove
+ (`!t. RED t ==> DEST_RED (MK_RED t) = t`,
+  REWRITE_TAC[DEST_MK_RED_EQ]);;
+
+let red_CASES = prove
+ (`!t. ?u. t = MK_RED u /\ RED u`,
+  MESON_TAC[red_tybij]);;
+
+let  FORALL_RED_THM = prove
+ (`!P. (!t. P t) <=> (!u. RED u ==> P (MK_RED u))`,
+  MESON_TAC[red_tybij]);;
+
+let  FORALL_RED_THM_IMP = prove
+ (`!P. (!u. RED u ==> P (MK_RED u)) ==> (!t. P t)`,
+  REWRITE_TAC[FORALL_RED_THM]);;
+
+let MK_RED_INJ_EQ = prove
+ (`!u u'. RED u /\ RED u' ==> (MK_RED u = MK_RED u' <=> u = u')`,
+  MESON_TAC[red_tybij]);;
+
+let MK_RED_INJ = prove
+ (`!u u'. RED u /\ RED u' /\ MK_RED u = MK_RED u' ==> u = u'`,
+  MESON_TAC[MK_RED_INJ_EQ]);;
+
+(* ------------------------------------------------------------------------- *)
+(* Substitution for the module of reductions.                                *)
+(* ------------------------------------------------------------------------- *)
+
+let TSUBST = new_definition
+  `TSUBST f t =
+   let x,y,r = DEST_RED t in
+   MK_RED (SUBST f x,SUBST f y,RSUBST f r)`;;
+
+let TSUBST_MK_RED = prove
+ (`!x y r f.
+     RED (x,y,r)
+     ==> TSUBST f (MK_RED (x,y,r)) = MK_RED (SUBST f x,SUBST f y,RSUBST f r)`,
+  REPEAT GEN_TAC THEN REWRITE_TAC[TSUBST] THEN LET_TAC THEN
+  ASM_METIS_TAC[PAIR_EQ; DEST_MK_RED]);;
+
+let RED_INVERSION = prove
+ (`(!x y. RED (x,y,LCREL_REFL x) <=> x = y) /\
+   (!x y r1 r2. RED (x,y,LCREL_TRANS r1 r2) <=>
+                (?z. RED (x,z,r1) /\ RED (z,y,r2))) /\
+   (!x y r1 r2.
+        RED (x,y,LCREL_APP r1 r2) <=>
+        (?x1 x2 y1 y2.
+           x = APP x1 x2 /\ y = APP y1 y2 /\
+           RED (x1,y1,r1) /\ RED (x2,y2,r2))) /\
+   (!x y r. RED (x,y,LCREL_ABS r) <=>
+            (?z w. x = ABS z /\ y = ABS w /\ RED (z,w,r))) /\
+   (!x y u v. RED (x,y,LCREL_BETA u v) <=>
+          x = APP (ABS u) v /\ y = SUBST (PUSHENV v REF) u) /\
+   (!x y. RED (x,y,LCREL_ETA u) <=>
+          x = ABS (APP (REINDEX SUC u) (REF 0)) /\ y = u)`,
+  REPEAT STRIP_TAC THEN GEN_REWRITE_TAC LAND_CONV [RED_CASES] THEN
+  REWRITE_TAC[PAIR_EQ; injectivity "lcrel"; distinctness "lcrel"] THEN
+  MESON_TAC[]);;
+
+let RED_SUBST = prove
+ (`!x y r f. RED (x,y,r) ==> RED (SUBST f x,SUBST f y,RSUBST f r)`,
+  REWRITE_TAC[RIGHT_FORALL_IMP_THM] THEN MATCH_MP_TAC RED_INDUCT_ALT THEN
+  REWRITE_TAC[SUBST; RSUBST; DERIV; SUBST_REINDEX; DERIV_O_SUC; RED_RULES] THEN
+  REWRITE_TAC[RED_INVERSION; injectivity "dblambda"; SUBST_SUBST;
+    SUBST_REINDEX; REINDEX_SUBST; GSYM CONJ_ASSOC; UNWIND_THM1;
+    RIGHT_EXISTS_AND_THM; SUBST_EXTENS; o_THM; SUBST_PUSHENV_LEMMA] THEN
+  MESON_TAC[]);;
+
+let TSUBST_TSUBST = prove
+ (`!f g t. TSUBST f (TSUBST g t) = TSUBST (SUBST f o g) t`,
+  GEN_TAC THEN GEN_TAC THEN MATCH_MP_TAC FORALL_RED_THM_IMP THEN
+  SIMP_TAC[FORALL_PAIR_THM; TSUBST_MK_RED; RED_SUBST; SUBST_SUBST; RSUBST_SUBST]);;
+
+let TSUBST_REF = prove
+ (`!t. TSUBST REF t = t`,
+  MATCH_MP_TAC FORALL_RED_THM_IMP THEN
+  SIMP_TAC[FORALL_PAIR_THM; TSUBST_MK_RED; RED_SUBST; SUBST_REF; RSUBST_REF]);;
+
+let MODULE_TSUBST = prove
+ (`MODULE SUBST TSUBST`,
+  REWRITE_TAC[MODULE_DEF; DBLAMBDA_DBMONAD; DBLAMBDA_DBUNIT;
+              TSUBST_REF; TSUBST_TSUBST]);;
+
+let TRED1 = new_definition
+  `TRED1 t = let x,y,r = DEST_RED t in x`;;
+
+let TRED2 = new_definition
+  `TRED2 t = let x,y,r = DEST_RED t in y`;;
+
+let TRED1_MK_RED = prove
+ (`!x y r. RED (x,y,r) ==> TRED1 (MK_RED (x,y,r)) = x`,
+  REPEAT STRIP_TAC THEN REWRITE_TAC[TRED1] THEN LET_TAC THEN
+  POP_ASSUM MP_TAC THEN ASM_SIMP_TAC[DEST_MK_RED; PAIR_EQ]);;
+
+let TRED2_MK_RED = prove
+ (`!x y r. RED (x,y,r) ==> TRED2 (MK_RED (x,y,r)) = y`,
+  REPEAT STRIP_TAC THEN REWRITE_TAC[TRED2] THEN LET_TAC THEN
+  POP_ASSUM MP_TAC THEN ASM_SIMP_TAC[DEST_MK_RED; PAIR_EQ]);;
+
+let TRED1_TSUBST = prove
+ (`!f t. TRED1 (TSUBST f t) = SUBST f (TRED1 t)`,
+  GEN_TAC THEN MATCH_MP_TAC FORALL_RED_THM_IMP THEN
+  SIMP_TAC[FORALL_PAIR_THM; TSUBST_MK_RED; TRED1_MK_RED; RED_SUBST]);;
+
+let TRED2_TSUBST = prove
+ (`!f t. TRED2 (TSUBST f t) = SUBST f (TRED2 t)`,
+  GEN_TAC THEN MATCH_MP_TAC FORALL_RED_THM_IMP THEN
+  SIMP_TAC[FORALL_PAIR_THM; TSUBST_MK_RED; TRED2_MK_RED; RED_SUBST]);;
+
+let MODULE_MOR_TRED1 = prove
+ (`MODULE_MOR SUBST TSUBST SUBST TRED1`,
+  REWRITE_TAC[MODULE_MOR; MODULE_TSUBST; MODULE_SUBST; TRED1_TSUBST]);;
+
+let MODULE_MOR_TRED2 = prove
+ (`MODULE_MOR SUBST TSUBST SUBST TRED2`,
+  REWRITE_TAC[MODULE_MOR; MODULE_TSUBST; MODULE_SUBST; TRED2_TSUBST]);;
+
+(* ------------------------------------------------------------------------- *)
+(* Reduction monads.                                                         *)
+(* ------------------------------------------------------------------------- *)
+
+let REDMONAD = new_definition
+  `REDMONAD (op,mop,p1,p2) <=>
+   MODULE_MOR op mop op p1 /\
+   MODULE_MOR op mop op p2`;;
+
+let REDMONAD_CLAUESES = prove
+ (`!op mop p1 p2:A->B.
+     REDMONAD (op,mop,p1,p2)
+     ==> DBMONAD op /\
+         MODULE op mop /\
+         MODULE_MOR op mop op p1 /\
+         MODULE_MOR op mop op p2`,
+  SIMP_TAC[REDMONAD; MODULE_MOR; MODULE_DEF]);;
+
+let REDMONAD_MOR = new_definition
+  `REDMONAD_MOR (op,mop,p1,(p2:M->A))
+                (op',mop',p1',(p2':N->B))
+                (f:A->B,g:M->N) <=>
+   REDMONAD (op,mop,p1,p2) /\
+   REDMONAD (op',mop',p1',p2') /\
+   DBMONAD_MOR op op' f /\
+   MODULE_MOR op mop (PBMOP op op' f mop') g /\
+   p1' o g = f o p1 /\
+   p2' o g = f o p2`;;
+
+(* ------------------------------------------------------------------------- *)
+(* Lambda calculus as reduction monad.                                       *)
+(* ------------------------------------------------------------------------- *)
+
+let REDMONAD_DBMONAD = prove
+ (`REDMONAD (SUBST,TSUBST,TRED1,TRED2)`,
+  REWRITE_TAC[REDMONAD; MODULE_MOR; MODULE_SUBST; MODULE_TSUBST;
+              TRED1_TSUBST; TRED2_TSUBST]);;
